
\begin{frame}[fragile]
\begin{minted}{haskell}
data Term = 
    TmFalse 
  | TmTrue 
  | TmOr Term Term 
\end{minted}
\end{frame}

\begin{frame}[fragile]
  \begin{minted}{haskell}
value :: Term -> Maybe Term
value TmFalse = 
  return TmFalse
value TmTrue  = 
  return TmTrue
value _       = 
  Nothing
  \end{minted}
\end{frame}

\begin{frame}[fragile]
  \begin{minted}{haskell}
step :: Term -> Maybe Term

step (TmOr TmFalse tm2) = 
  return tm2

step (TmOr TmTrue  tm2) = 
  return TmTrue

step (TmOr tm1     tm2) = do
  tm1' <- step tm1
  return $ TmOr tm1' tm2

step _                  =
  Nothing
  \end{minted}
\end{frame}
