
\begin{frame}[fragile]
  \begin{minted}{haskell}
data Term =
    TmInt Int
  | TmAdd Term Term
  \end{minted}
\end{frame}

\begin{frame}[fragile]
  \begin{minted}{haskell}
value :: Term -> Maybe Term
value (TmInt i) = Just (TmInt i)
value _         = Nothing
  \end{minted}
\end{frame}

\begin{frame}[fragile]
  \begin{minted}{haskell}
step :: Term -> Maybe Term

step (TmAdd (TmInt i1) (TmInt i2)) = 
  return $ TmInt (i1 + i2)

step (TmAdd (TmInt i1) t2) = do
  t2' <- step t2
  return $ TmAdd (TmInt i1) t2'

step (TmAdd t1 t2) =  do
  t1' <- step t1
  return $ TmAdd t1' t2

step _ = Nothing
  \end{minted}
\end{frame}

\begin{frame}[fragile]
  \begin{minted}{haskell}
eval :: Term -> Maybe Term

eval tm = 
  case step tm of
    Just tm' -> eval tm
    Nothing  -> value tm
  \end{minted}
\end{frame}

\begin{frame}[fragile]
  \begin{mdframed}[frametitle={Previously...}]
\begin{minted}{haskell}
step :: Term -> Maybe Term
step (TmAdd (TmInt i1) (TmInt i2)) = -- E-AddInt
  return $ TmInt (i1 + i2)
...
step (TmAdd t1 t2) =  do             -- E-Add1
  t1' <- step t1
  return $ TmAdd t1' t2
...
\end{minted}
  \end{mdframed}
  \vfill
\begin{minted}{haskell}
> step $
    TmAdd 
      (TmAdd (TmInt 1) (TmInt 2)) 
      (TmAdd (TmInt 3) (TmInt 4))
Just $ 
  TmAdd 
    (TmInt 3) 
    (TmAdd (TmInt 3) (TmInt 4))
\end{minted}
\end{frame}
