
\section{Natural deduction rules}

\begin{frame}[c]
  We use natural deduction style rules for most of this.
\end{frame}

\begin{frame}
  \infrule[Rule-Name]
          {Assumption_1 \andalso Assumption_2 \andalso \ldots}
          {Conclusion}
\end{frame}

\begin{frame}[c]
  \begin{mdframed}[frametitle={Rules for evenness}]

  \infrule[Even-Zero]
          {}
          {\text{even}~0}
  \infrule[Even-Add]
          {\text{even}~x}
          {\text{even}~\left(x + 2\right)}
  \end{mdframed}

  \medskip

  \begin{overprint}
  \onslide<+>
  Some rules - like $\text{Even-Zero}$ - have no assumptions, and are known as {\it axioms}.
  \onslide<+>
  Some rules - like $\text{Even-Add}$ - are recursive.
  \onslide<+>
  The relations are determined by the union of all of the rules.
  \onslide<+>
  Usually only one rule will apply at one time, and so the order we organize these rules in doesn't matter.
  \onslide<+>
  We are also dealing with an "open world".
  \onslide<+>
  Rules will often get added to a system without having to go back and alter the other rules.
  \end{overprint}
\end{frame}

\begin{frame}[c]
  \begin{mdframed}[frametitle={Rules for evenness, now with bonus rules}]

  \infrule[Even-Zero]
          {}
          {\text{even}~0}
  \infrule[Even-Add]
          {\text{even}~x}
          {\text{even}~\left(x + 2\right)}
  \infrule[Even-Odd]
          {\text{odd}~x}
          {\text{even}~\left(x + 1\right)}
  \infrule[Odd-Even]
          {\text{even}~x}
          {\text{odd}~\left(x + 1\right)}
  \end{mdframed}

  \medskip

  \begin{overprint}
  \onslide<+>
  Let us add some more rules.
  \onslide<+>
  Now we could apply these rules in a few different orders to determine $\text{even 4}$.
  \onslide<+>
  We want the rules to be {\it deterministic} - the answers through all of the paths agree, and the paths are finite.
  \end{overprint}
\end{frame}

\begin{frame}[c]
  \begin{mdframed}[frametitle={Equivalence relations}]

  \infrule[Reflexivity]
          {}
          {P = P}
  \infrule[Symmetry]
          {Q = P}
          {P = Q}
  \infrule[Transitivity]
          {P = Q \andalso Q = R}
          {P = R}
  \end{mdframed}

  \medskip

  \begin{overprint}
  \onslide<+>
  Sometimes we have rules like $\text{Symmetry}$, which could be applied over and over and spin forever.
  \onslide<+>
  Those rules usually exist in that form to explain why a system has some desired properties, or to assist with proofs.
  \onslide<+>
  There will often be a second equivalent set of rules applied that are deterministic and terminating - known as {\i algorithmic} to assist with implementations.
  \onslide<+>
  This is usually proved by a proof of logical equivalence of the non-deterministic and algorithmic rules sets.
  \end{overprint}
\end{frame}

\begin{frame}[fragile]
  \begin{minted}{haskell}
class Applicative f => Alternative f where
  empty :: f a
  (<|>) :: f a -> f a -> f a
  \end{minted}
\end{frame}

\begin{frame}[fragile]
  \onslide<+->
  \begin{minted}{haskell}
> Nothing <|> Nothing
  \end{minted}
  \onslide<+->
  \begin{minted}{haskell}
Nothing
  \end{minted}
  \onslide<+->
  \begin{minted}{haskell}
> Just 1 <|> Nothing
  \end{minted}
  \onslide<+->
  \begin{minted}{haskell}
Just 1
  \end{minted}
  \onslide<+->
  \begin{minted}{haskell}
> Nothing <|> Just 2
  \end{minted}
  \onslide<+->
  \begin{minted}{haskell}
Just 2
  \end{minted}
  \onslide<+->
  \begin{minted}{haskell}
> Just 1 <|> Just 2
  \end{minted}
  \onslide<+->
  \begin{minted}{haskell}
Just 1
  \end{minted}
\end{frame}

\begin{frame}[fragile]
  \begin{minted}{haskell}
asum :: (Foldable t, Alternative f) => t (f a) -> f a 
asum = foldr (<|>) empty
  \end{minted}
\end{frame}

\begin{frame}[fragile]
  \begin{minted}{haskell}
> asum [Just 1, Just 2, Just 3]
  \end{minted}
  \onslide<+->
  \begin{minted}{haskell}
Just 1
  \end{minted}
  \onslide<+->
  \begin{minted}{haskell}
> asum [Nothing, Just 2, Just 3]
  \end{minted}
  \onslide<+->
  \begin{minted}{haskell}
Just 2
  \end{minted}
  \onslide<+->
  \begin{minted}{haskell}
> asum [Nothing, Nothing, Nothing]
  \end{minted}
  \onslide<+->
  \begin{minted}{haskell}
Nothing
  \end{minted}
  \onslide<+->
  \begin{minted}{haskell}
> asum []
  \end{minted}
  \onslide<+->
  \begin{minted}{haskell}
Nothing
  \end{minted}
\end{frame}

\begin{frame}[fragile]
  \onslide<+->
  \begin{minted}{haskell}
type RuleSet a b = a -> Maybe b
  \end{minted}

  \onslide<+->
  \begin{minted}{haskell}
type Rule a b = RuleSet a b -> a -> Maybe b
  \end{minted}

  \onslide<+->
  \begin{minted}{haskell}
mkRuleSet :: [Rule a b] -> RuleSet a b
  \end{minted}

  \onslide<+->
  \begin{minted}{haskell}
mkRuleSet rules =
  let
    ruleSet a =
      asum .
      fmap (\r -> r ruleSet a) $
      rules
  in
    ruleSet
  \end{minted}
\end{frame}

\begin{frame}[fragile]
  \begin{columns}
    \begin{column}{0.5\textwidth}
      \begin{minted}{haskell}
evenZero :: Rule Int ()
evenZero _ x
  | x == 0 = Just ()
  | otherwise = Nothing
      \end{minted}
    \end{column}
    \begin{column}{0.5\textwidth}
  \infrule[Even-Zero]
          {}
          {\text{even}~0}
    \end{column}
  \end{columns}
\end{frame}

\begin{frame}[fragile]
  \begin{columns}
    \begin{column}{0.5\textwidth}
      \begin{minted}{haskell}
evenAddTwo :: Rule Int ()
evenAddTwo e n
  | n >= 2 = e (n - 2)
  | otherwise = Nothing
      \end{minted}
    \end{column}
    \begin{column}{0.5\textwidth}
  \infrule[Even-Add]
          {\text{even}~x}
          {\text{even}~\left(x + 2\right)}
    \end{column}
  \end{columns}
\end{frame}

\begin{frame}[fragile]
  \begin{minted}{haskell}
evenR :: RuleSet Int ()
evenR = mkRuleSet [evenZero, evenAddTwo]
  \end{minted}
\end{frame}

\begin{frame}[fragile,c]
  \begin{columns}
    \begin{column}{0.5\textwidth}
  \begin{minted}{haskell}
evenOdd :: RuleSet Int () -> Rule Int ()
evenOdd o _ n
  | n >= 1 = o (n - 1)
  | otherwise = Nothing
  \end{minted}
    \end{column}
    \begin{column}{0.5\textwidth}
  \infrule[Even-Odd]
          {\text{odd}~x}
          {\text{even}~\left(x + 1\right)}
    \end{column}
  \end{columns}
\end{frame}

\begin{frame}[fragile]
  \begin{columns}
    \begin{column}{0.5\textwidth}
  \begin{minted}{haskell}
oddEven :: RuleSet Int () -> Rule Int ()
oddEven e _ n
  | n >= 1 = e (n - 1)
  | otherwise = Nothing
  \end{minted}
    \end{column}
    \begin{column}{0.5\textwidth}
  \infrule[Odd-Even]
          {\text{even}~x}
          {\text{odd}~\left(x + 1\right)}
    \end{column}
  \end{columns}
\end{frame}


\begin{frame}[fragile]
  \begin{minted}{haskell}
evenR, oddR :: RuleSet Int ()
evenR = mkRuleSet [evenZero, evenOdd oddR]
oddR  = mkRuleSet [oddEven evenR]
  \end{minted}
\end{frame}

\begin{frame}[fragile]
  \begin{minted}{haskell}
evenR, oddR :: RuleSet Int ()
evenR = mkRuleSet [evenZero, evenAddTwo, evenOdd oddR]
oddR  = mkRuleSet [oddEven evenR]
  \end{minted}
\end{frame}

\begin{frame}[fragile]
  \onslide<+->
  \begin{minted}{haskell}
> evenR 3
  \end{minted}
  \onslide<+->
  \begin{minted}{haskell}
Nothing
  \end{minted}

  \onslide<+->
  \begin{minted}{haskell}
> evenR 4
  \end{minted}
  \onslide<+->
  \begin{minted}{haskell}
Just ()
  \end{minted}

  \onslide<+->
  \begin{minted}{haskell}
> oddR 3
  \end{minted}
  \onslide<+->
  \begin{minted}{haskell}
Just ()
  \end{minted}

  \onslide<+->
  \begin{minted}{haskell}
> oddR 4
  \end{minted}
  \onslide<+->
  \begin{minted}{haskell}
Nothing
  \end{minted}
\end{frame}
